template-coq/theories/MetaTheory.v
@@ -10,21 +10,21 @@ Set Asymmetric Patterns.
 Existing Instance config.default_checker_flags.
 
 (** Use a coercion for this common projection of the global context. *)
-Definition fst_ctx : global_context -> global_declarations := fst.
-Coercion fst_ctx : global_context >-> global_declarations.
+Definition fst_ctx : global_env_ext -> global_env := fst.
+Coercion fst_ctx : global_env_ext >-> global_env.
 
 (** The subject reduction property of the system.
     We comment this as otherwise extraction can produce "axioms to be realized"
     values that make extracted code useless, as type are in Type.
  *)
 (*
-Conjecture subject_reduction : forall (Σ : global_context) Γ t u T,
+Conjecture subject_reduction : forall (Σ : global_env_ext) Γ t u T,
     Σ ;;; Γ |- t : T -> red Σ Γ t u -> Σ ;;; Γ |- u : T.
 *)
 (** Weak Normalization: every term has a normal form *)
 
-Definition normal (Σ : global_context) Γ t := { u & red1 Σ Γ t u } -> False.
+Definition normal (Σ : global_env_ext) Γ t := { u & red1 Σ Γ t u } -> False.
 (*
-Conjecture weak_normalization : forall (Σ : global_context) Γ t T,
+Conjecture weak_normalization : forall (Σ : global_env_ext) Γ t T,
     Σ ;;; Γ |- t : T -> { u & (red Σ Γ t u * normal Σ Γ u)%type }.
 *)
