test-suite/TypingTests.v
@@ -43,8 +43,8 @@ Ltac infer := try red;
 
 Quote Definition natr := nat.
 
-Definition type_program (p : global_declarations * term) (ty : term) :=
-  let Σ := reconstruct_global_context (fst p) in
+Definition type_program (p : program) (ty : term) :=
+  let Σ := empty_ext (fst p) in
   Σ ;;; [] |- snd p : ty.
 
 Example typecheck_four : type_program four natr:= ltac:(typecheck).
@@ -59,7 +59,7 @@ Qed.
 (* Eval native_compute in typecheck_program p_Plus1. *)
 
 Definition test_reduction (p : program) :=
-    let Σ := reconstruct_global_context (fst p) in
+    let Σ := empty_ext (fst p) in
     reduce (fst Σ) [] (snd p).
 
 Definition string_of_env_error e :=
@@ -159,11 +159,11 @@ Definition f2 := (forall (A:Type@{i}) (B: Prop), A -> B -> B).
 
 Quote Definition f1' := (forall (A:Type@{i}) (B: Prop), A -> B -> A). 
 
-Eval lazy in infer' (nil, ConstraintSet.empty) nil f1'.
+Eval lazy in infer' (empty_ext []) nil f1'.
 
 Quote Definition f2' := (forall (A:Type@{i}) (B: Prop), A -> B -> B). 
 
-Eval lazy in infer' (nil, ConstraintSet.empty) nil f2'.
+Eval lazy in infer' (empty_ext []) nil f2'.
 
 Definition f := (forall (A:Type@{i}) (B: Type@{j}), A -> B -> A).
 (* : Type@{i+1, j+1} *)
@@ -172,4 +172,4 @@ Quote Definition f' := (forall (A:Type@{i}) (B:Type@{j}), A -> B -> A).
 
 Quote Definition f'' := (forall (B: Type@{j}), B -> B). 
 
-Eval lazy in infer' (nil, ConstraintSet.empty) nil f'.
+Eval lazy in infer' (empty_ext []) nil f'.
